auto-theories/Signatures.v
@@ -1,0 +1,9 @@
+Require Import Cpp.Auto.
+
+(* signatures
+ * note(gmm): these should be moved out to cpp2v
+ *)
+Definition signature := list (obj_name * function_spec).
+
+Definition sig {resolve} (ti : thread_info) (s : signature) : mpred :=
+  sepSPs (map (fun '(f, fs) => cglob (resolve:=resolve) f ti fs) s).
